list_vector/ListVectorSpec.v
@@ -1,27 +1,303 @@
 Require Fin List.
 Require Import ListVectorDef PeanoNat Eqdep_dec.
 Import ListVectorNotations EqNotations.
+Require Import Lia.
 
-Lemma eq_iff_elts_eq A n (v1 v2: t A n):
-  v1 = v2 <-> elts v1 = elts v2.
-split.
-- intros.
-  now rewrite H.
-- intros.
-  destruct v1 as [el_v1 sp_v1].
-  destruct v2 as [el_v2 sp_v2].
-  cbn in *.
-  
+Definition cons_inj {A} {a1 a2} {n} {v1 v2 : t A n}
+ (eq : a1 :: v1 = a2 :: v2) : a1 = a2 /\ v1 = v2 :=
+conj 
+  (f_equal hd eq)
+  (proj1 (vec_spec_eq v1 v2) (f_equal elts (f_equal tl eq))).
+
+Lemma nil_spec {A} (v : t A 0) : v = [].
+Proof.
+apply (fun P E => case0 P E v). reflexivity.
+Defined.
 
 Lemma eq_nth_iff A n (v1 v2: t A n):
   (forall p1 p2, p1 = p2 -> v1 [@ p1 ] = v2 [@ p2 ]) <-> v1 = v2.
 Proof.
 split.
-- intros.
-  destruct v1 as [el_v1 sp_v1], v2 as [el_v2 sp_v2].
-  enough (el_v1 = el_v2 /\ sp_v1 = sp_v2).
-  
+- revert n v1 v2; refine (@rect2 _ _ _ _ _).
+  + reflexivity.
+  + intros n ? ? H ? ? H0. f_equal.
+    * apply (H0 Fin.F1 Fin.F1 eq_refl).
+    * apply H. 
+      intros p1 p2 H1.
+      specialize (H0 (Fin.FS p1) (Fin.FS p2) (f_equal (@Fin.FS n) H1)).
+      destruct v1, v2.
+      cbn in H0.
+      enough ({| elts := elts; elts_spec := f_equal Init.Nat.pred (f_equal S elts_spec) |} = {| elts := elts; elts_spec := elts_spec |} /\ {| elts := elts0; elts_spec := f_equal Init.Nat.pred (f_equal S elts_spec0) |} = {| elts := elts0; elts_spec := elts_spec0 |}).
+      -- destruct H2.
+        rewrite <- H2.
+        rewrite <- H3.
+        apply H0.
+      -- split; apply vec_spec_eq; reflexivity.
+- intros; now f_equal.
+Qed.
+
+Lemma eta {A} {n} (v : t A (S n)) : v = hd v :: tl v.
+Proof.
+apply (fun P IS => caseS P IS (n := n) v). 
+intros. 
+apply vec_spec_eq.
+reflexivity.
+Defined.
+
+Lemma replace_id A: forall n p (v : t A n),
+  replace v p (nth v p) = v.
+Proof.
+intros n p.
+induction p as [|? p IHp].
+- intros v.
+  rewrite (eta v).
+  cbn.
+  apply vec_spec_eq.
+  cbn.
+  reflexivity.
+- intros v.
+  rewrite (eta v).
+  cbn.
+  apply vec_spec_eq.
+  cbn.
+
+intros n p; induction p as [|? p IHp]; intros v; rewrite (eta v); simpl; apply vec_spec_eq; [reflexivity|].
+now rewrite IHp.
+Qed.
+
+Lemma replace_replace_eq A: forall n p (v : t A n) a b,
+  replace (replace v p a) p b = replace v p b.
+Proof.
+intros n p v a b.
+induction p as [|? p IHp]; rewrite (eta v); simpl; [reflexivity|].
+now rewrite IHp.
+Qed.
 
 
-Lemma nth_ext : forall l l' d d', length l = length l' ->
-  (forall n, n < length l -> nth n l d = nth n l' d') -> l = l'.
+Lemma const_nth A (a: A) n (p: Fin.t n): (const a n)[@ p] = a.
+Proof.
+now induction p.
+Qed.
+
+
+Lemma append_const A (a : A) n m : (const a n) ++ (const a m) = const a (n + m).
+Proof.
+induction n as [|n IH].
+- reflexivity.
+- cbn. apply f_equal, IH.
+Qed.
+
+Lemma map_id A: forall n (v : t A n),
+  map (fun x => x) v = v.
+Proof.
+intros n v; induction v as [|? ? v IHv]; simpl; [ | rewrite IHv ]; auto.
+Qed.
+
+Lemma map_map A B C: forall (f:A->B) (g:B->C) n (v : t A n),
+  map g (map f v) = map (fun x => g (f x)) v.
+Proof.
+intros f g n v; induction v as [|? ? v IHv]; simpl; [ | rewrite IHv ]; auto.
+Qed.
+
+Lemma map_append A B: forall (f:A->B) n m (v: t A n) (w: t A m),
+  (map f (v ++ w)) = map f v ++ map f w.
+Proof.
+intros f n m v w. induction v as [|? ? v IHv].
+- reflexivity.
+- cbn. apply f_equal, IHv.
+Qed.
+
+Lemma take_O : forall {A} {n} le (v:t A n), take 0 le v = [].
+Proof.
+  reflexivity.
+Qed.
+
+
+Lemma take_idem : forall {A} p n (v:t A n) le le',
+  take p le' (take p le v) = take p le v.
+Proof.
+  intros A p; induction p as [|p IHp]; intros n v le le'.
+  - reflexivity.
+  - destruct v.
+    + inversion le.
+    + simpl. apply f_equal, IHp.
+Qed.
+
+Lemma append_comm_cons {A} : forall {n m : nat} (v : t A n) (w : t A m) (a : A),
+  a :: (v ++ w) = (a :: v) ++ w.
+Proof. reflexivity. Qed.
+
+Locate "rew".
+
+Lemma rev_cons A: forall a n (v : t A n), rev (a :: v) = shiftin a (rev v).
+Proof.
+intros a n v. unfold rev, rev_append, eq_rect_r.
+rewrite !rew_compose.
+enough (H : forall m (w : t A m) k (E1 : _ = k) E2,
+  rew [t A] E2 in rev_append_tail v (shiftin a w) =
+  shiftin a (rew [t A] E1 in rev_append_tail v w)) by apply (H 0 []).
+induction v as [|b n v IH]; intros m w k E1 E2; cbn.
+- subst k. now rewrite (UIP_refl_nat _ E2).
+- apply (IH _ (b :: w)).
+Qed.
+
+Lemma splitat_append {A} : forall {n m : nat} (v : t A n) (w : t A m),
+  splitat n (v ++ w) = (v, w).
+Proof.
+  intros n m v w. induction v as [|a n v IH].
+  - reflexivity.
+  - cbn. now rewrite IH.
+Qed.
+
+Lemma append_inj {A} : forall {n m : nat} (v v' : t A n) (w w' : t A m),
+  v ++ w = v' ++ w' -> v = v' /\ w = w'.
+Proof.
+intros n m v v' w w' E%(f_equal (splitat _)).
+apply pair_equal_spec.
+now rewrite <- !splitat_append.
+Qed.
+
+Lemma rev_nil A: rev (nil A) = [].
+Proof.
+unfold rev, rev_append.
+now rewrite (UIP_refl_nat _ (plus_n_O 0)), (UIP_refl_nat _ (Nat.tail_add_spec 0 0)).
+Qed.
+
+Lemma rev_shiftin A: forall a n (v : t A n),
+  rev (shiftin a v) = a :: rev v.
+Proof.
+intros a n v. induction v as [|b n v IH]; cbn.
+- now rewrite rev_cons, !rev_nil.
+- now rewrite !rev_cons, IH.
+Qed.
+
+Lemma rev_rev A: forall n (v : t A n), rev (rev v) = v.
+Proof.
+intros n v. induction v as [|a n v IH].
+- now rewrite !rev_nil.
+- now rewrite rev_cons, rev_shiftin, IH.
+Qed.
+
+Lemma map_shiftin A B: forall (f : A -> B) a n (v : t A n),
+  map f (shiftin a v) = shiftin (f a) (map f v).
+Proof.
+intros f a n v. induction v as [|b n v IH].
+- reflexivity.
+- cbn. apply f_equal, IH.
+Qed.
+
+Lemma map_rev A B: forall (f : A -> B) n (v : t A n),
+  map f (rev v) = rev (map f v).
+Proof.
+intros f n v. induction v as [|a n v IH]; cbn.
+- now rewrite !rev_nil.
+- now rewrite !rev_cons, map_shiftin, IH.
+Qed.
+
+Lemma to_list_of_list_opp {A} (l: list A): to_list (of_list l) = l.
+Proof.
+induction l.
+- reflexivity.
+- unfold to_list; simpl. now f_equal.
+Qed.
+
+
+Lemma length_to_list A n (v : t A n): length (to_list v) = n.
+Proof. induction v; cbn; auto. Qed.
+
+Lemma of_list_to_list_opp A n (v: t A n):
+  rew length_to_list _ _ _ in of_list (to_list v) = v.
+Proof.
+induction v as [ | h n v IHv ].
+- now apply case0 with (P := fun v => v = nil A).
+- replace (length_to_list _ _ (cons _ h _ v)) with (f_equal S (length_to_list _ _ v))
+    by apply (UIP_dec Nat.eq_dec).
+  cbn; rewrite map_subst_map.
+  f_equal.
+  now etransitivity; [ | apply IHv].
+Qed.
+
+Lemma to_list_nil A : to_list (nil A) = List.nil.
+Proof. reflexivity. Qed.
+
+Lemma to_list_cons A h n (v : t A n):
+  to_list (cons A h n v) = List.cons h (to_list v).
+Proof. reflexivity. Qed.
+
+Lemma to_list_nil_iff A v:
+  to_list v = List.nil <-> v = nil A.
+Proof.
+split; intro H.
+- now apply case0 with (P := fun v => v = []).
+- subst. apply to_list_nil.
+Qed.
+
+
+Lemma to_list_inj A n (v w : t A n):
+  to_list v = to_list w -> v = w.
+Proof.
+revert v. induction w as [| w0 n w IHw].
+- apply to_list_nil_iff.
+- intros v H. rewrite (eta v) in H.
+  injection H as [=H0 H1%IHw]. subst. apply eta.
+Qed.
+
+Lemma to_list_hd A n (v : t A (S n)) d:
+  hd v = List.hd d (to_list v).
+Proof. now rewrite (eta v). Qed.
+
+Lemma to_list_last A n (v : t A (S n)) d:
+  last v = List.last (to_list v) d.
+Proof.
+apply rectS with (v:=v); [reflexivity|].
+intros a k u IH.
+rewrite to_list_cons.
+simpl List.last.
+now rewrite <- IH, (eta u).
+Qed.
+
+Lemma to_list_const A (a : A) n:
+  to_list (const a n) = List.repeat a n.
+Proof.
+induction n as [ | n IHn ]; [reflexivity|].
+now cbn; rewrite <- IHn.
+Qed.
+
+Lemma to_list_tl A n (v : t A (S n)):
+  to_list (tl v) = List.tl (to_list v).
+Proof. now rewrite (eta v). Qed.
+
+Lemma to_list_append A n m (v1 : t A n) (v2 : t A m):
+  to_list (append v1 v2) = List.app (to_list v1) (to_list v2).
+Proof.
+induction v1; simpl; trivial.
+now rewrite to_list_cons; f_equal.
+Qed.
+
+Lemma to_list_rev_append_tail A n m (v1 : t A n) (v2 : t A m):
+  to_list (rev_append_tail v1 v2) = List.rev_append (to_list v1) (to_list v2).
+Proof. now revert m v2; induction v1 as [ | ? ? ? IHv1 ]; intros; [ | simpl; rewrite IHv1 ]. Qed.
+
+Lemma to_list_rev_append A n m (v1 : t A n) (v2 : t A m):
+  to_list (rev_append v1 v2) = List.rev_append (to_list v1) (to_list v2).
+Proof. unfold rev_append; rewrite <- (Nat.tail_add_spec n m); apply to_list_rev_append_tail. Qed.
+
+Lemma to_list_rev A n (v : t A n):
+  to_list (rev v) = List.rev (to_list v).
+Proof.
+unfold rev; rewrite (plus_n_O n); unfold eq_rect_r; simpl.
+now rewrite to_list_rev_append, List.rev_alt.
+Qed.
+
+Lemma to_list_map A B (f : A -> B) n (v : t A n) :
+  to_list (map f v) = List.map f (to_list v).
+Proof.
+induction v; cbn; [reflexivity|].
+now cbn; f_equal.
+Qed.
+
+Lemma to_list_fold_right A B f (b : B) n (v : t A n):
+  fold_right f v b = List.fold_right f b (to_list v).
+Proof. now revert b; induction v; cbn; intros; f_equal. Qed.
+
+
