utils/list_utils.v
@@ -1,5 +1,16 @@
 Require Import List.
 Require Import Lia.
+Import ListNotations.
+
+Lemma list_eq_cons {A:Type}: forall {a1 a2:A} (l1 l2:list A), a1 = a2 /\ l1 = l2 -> a1 :: l1 = a2 :: l2.
+Proof.
+intros a1 a2 l1 l2 H.
+destruct H.
+rewrite H.
+rewrite H0.
+reflexivity.
+Qed.
+
 Fixpoint list_replace {A:Type} (l:list A) (n:nat) (a:A) : list A := 
 match l with
 | Datatypes.nil => Datatypes.nil
