coq_vector_comparison_notes/progress.md
@@ -1,0 +1,67 @@
+# Progress Lemma implementation
+## functional
+- [x] eq_nth_iff
+
+## list 
+- [x] eq_nth_iff
+
+## recursive
+- [x] eq_nth_iff
+
+# Progress function implementation
+
+## functinal 
+- [x] nil
+- [x] cons
+- [x] vector_ind
+- [x] hd
+- [x] tl
+- [x] last
+- [x] const
+- [x] nth
+- [x] replace
+- [x] take
+- [x] append
+- [x] rev
+- [x] map
+- [x] fold_right
+- [x] of_list
+- [x] to_list
+
+
+
+## list 
+- [x] nil
+- [x] cons
+- [x] vector_ind
+- [x] hd
+- [x] tl
+- [x] last
+- [x] const
+- [x] nth
+- [x] replace
+- [x] take
+- [x] append
+- [x] rev
+- [x] map
+- [x] fold_right
+- [x] of_list
+- [x] to_list
+
+## recursive 
+- [x] nil
+- [x] cons
+- [x] vector_ind
+- [x] hd
+- [x] tl
+- [x] last
+- [x] const
+- [x] nth
+- [x] replace
+- [x] take
+- [x] append
+- [x] rev
+- [x] map
+- [x] fold_right
+- [x] of_list
+- [x] to_list
