functional_vector/FunctionalVector.v
@@ -1,0 +1,4 @@
+Require FunctionalVectorDef.
+Require FunctionalVectorSpec.
+Include FunctionalVectorDef.
+Include FunctionalVectorSpec.
