list_vector/ListVector.v
@@ -1,0 +1,4 @@
+Require ListVectorDef.
+Require ListVectorSpec.
+Include ListVectorDef.
+Include ListVectorSpec.
